fixes

proof/memory_map.bpl
@@ -1,6 +1,7 @@
 var mem: mem_t;
 
-const NULL: uint8_ptr_t; axiom NULL == 0bv64;
+const NULL: uint8_ptr_t;
+axiom NULL == 0bv64;
 
 /*
 static sir_channel_context_t sir_channel_context;
@@ -9,10 +10,10 @@ const static_sir_channel_context_base_ptr : uint8_ptr_t;
 axiom static_sir_channel_context_base_ptr == 40960bv64;
 
 const stack_ptr_low: uint8_ptr_t;
-axiom stack_ptr_low == 4096bv64;
+axiom stack_ptr_low == 8192bv64;
 
 const stack_ptr_high: uint8_ptr_t;
-axiom stack_ptr_high == 8192bv64;
+axiom stack_ptr_high == 12288bv64;
 
 function {:inline} AddrInStack(rsp: bv64): bool
 {
@@ -20,13 +21,13 @@ function {:inline} AddrInStack(rsp: bv64): bool
 }
 
 const stack_guard_ptr_low: uint8_ptr_t;
-axiom stack_guard_ptr_low == 8192bv64;
+axiom stack_guard_ptr_low == 4096bv64;
 
 const stack_guard_ptr_high: uint8_ptr_t;
-axiom stack_guard_ptr_high == 12288bv64;
+axiom stack_guard_ptr_high == 8192bv64;
 
 const send_buf_ptr_low: uint8_ptr_t;
-axiom send_buf_ptr_low == 409600bv64;
+axiom send_buf_ptr_low == 417792bv64;
 const send_buf_size: uint64_t;
 axiom send_buf_size == 4096bv64;
 
@@ -37,3 +38,33 @@ axiom recv_buf_size == 4096bv64;
 
 const symmetric_key_ptr_low: uint8_ptr_t;
 axiom symmetric_key_ptr_low == 45056bv64;
+
+const U_ptr_low: uint8_ptr_t;
+axiom U_ptr_low == 368640bv64;
+const U_ptr_high : uint8_ptr_t;
+axiom U_ptr_high == 409600bv64;
+
+const SIR_ptr_low: uint8_ptr_t;
+axiom SIR_ptr_low == 0bv64;
+const SIR_ptr_high : uint8_ptr_t;
+axiom SIR_ptr_high == 409600bv64;
+
+function {:inline} AddrInU(ptr: bv64): bool
+{
+  GE_64(ptr, U_ptr_low) && LT_64(ptr, U_ptr_high)
+}
+
+function {:inline} AddrInSIR(ptr: bv64): bool
+{
+  GE_64(ptr, SIR_ptr_low) && LT_64(ptr, SIR_ptr_high)
+}
+
+function {:inline} get_send_buf_current(mem: mem_t): uint8_ptr_t
+{
+  LOAD_LE_64(mem, PLUS_64(static_sir_channel_context_base_ptr, 16bv64))
+}
+
+function {:inline} AddrInSendBuf(ptr: bv64): bool
+{
+  GE_64(ptr, send_buf_ptr_low) && LT_64(ptr, PLUS_64(send_buf_ptr_low, send_buf_size))
+}
