proof/verified_L.bpl
@@ -3,19 +3,22 @@ modifies mem;
 {
   var buf: uint8_ptr_t;
   var size: uint64_t;
+  var channel_result : channel_api_result_t;
 
   call init_channel(send_buf_ptr_low, send_buf_size,
                     recv_buf_ptr_low, recv_buf_size,
                     symmetric_key_ptr_low);
+                    
   while(*)
+  invariant AddrInSendBuf(get_send_buf_current(mem));
   {
     havoc buf;
     havoc size;
 
     if (*) { call U(); }
-    else if (*) { call L_malloc(size); }
-    else if (*) { call L_free(buf); }
-    else if (*) { call L_send(buf,size); }
-    else if (*) { call L_recv(buf,size); }
+    //else if (*) { call L_malloc(size); }
+    //else if (*) { call L_free(buf); }
+    else if (*) { call channel_result := L_send(buf,size); }
+    //else if (*) { call channel_result := L_recv(buf,size); }
   }
 }
